cava/cava/Cava/Arrow/ExprSemantics.v
@@ -14,10 +14,9 @@
 (* limitations under the License.                                           *)
 (****************************************************************************)
 
-From Arrow Require Import Category Arrow .
+From Arrow Require Import Category Arrow.
 From Cava Require Import Arrow.CavaArrow.
-From Cava Require Arrow.CombinationalArrow .
-(* From Cava Require Arrow.CombinationalArrow Arrow.EvaluationArrow. *)
+From Cava Require Import Arrow.CircuitSemantics.
 
 From Cava Require Import Arrow.ExprSyntax.
 From Cava Require Import Arrow.ExprLowering.
@@ -30,30 +29,31 @@ Local Open Scope category_scope.
 Local Open Scope arrow_scope.
 
 Section combinational_semantics.
-  Import Arrow.CombinationalArrow.
-  
   Definition coq_func i o := denote_kind i -> denote_kind o.
 
-  Fixpoint interp_combinational {i o: Kind}
+  Fixpoint interp_combinational' {i o: Kind}
     (expr: kappa coq_func i o)
     : denote_kind i -> (denote_kind o) :=
     match expr with
-    | Var x => fun v => (x v) 
-    | Abs f => fun '(x,y) => interp_combinational (f (fun _ => x)) y
-    | App f e => fun y => 
-      (interp_combinational f) (interp_combinational e tt, y)
-    | Comp g f => fun x => interp_combinational g (interp_combinational f x)
+    | Var x => fun v => (x v)
+    | Abs f => fun '(x,y) => interp_combinational' (f (fun _ => x)) y
+    | App f e => fun y =>
+      (interp_combinational' f) (interp_combinational' e tt, y)
+    | Comp g f => fun x => interp_combinational' g (interp_combinational' f x)
     | Primitive p => combinational_evaluation' (CavaArrow.Primitive p)
     | Id _ => fun x => x
-    | Let v f => fun y => 
-      interp_combinational (f (fun _ => interp_combinational v tt)) y
+    | Let v f => fun y =>
+      interp_combinational' (f (fun _ => interp_combinational' v tt)) y
     | LetRec v f => fun _ => kind_default _
     end.
-    
-    Axiom expression_evaluation_is_arrow_evaluation: forall i o (expr: Kappa i o), forall (x: denote_kind i),
-      combinational_evaluation' (closure_conversion 
-        
-        expr) x =
-      interp_combinational (expr _) x.
+
+  Definition interp_combinational {x y: Kind}
+    (expr: kappa coq_func x y)
+    (i: denote_kind (remove_rightmost_unit x)): (denote_kind y) :=
+    interp_combinational' expr (apply_rightmost_tt x i).
+
+  Axiom expression_evaluation_is_arrow_evaluation: forall i o (expr: Kappa i o), forall (x: denote_kind i),
+    combinational_evaluation' (closure_conversion expr) x =
+    interp_combinational' (expr _) x.
 
 End combinational_semantics.
