cava/cava/Cava/Arrow/ExprEquiv.v
@@ -1,14 +1,10 @@
 From Coq Require Import List PeanoNat Arith.Peano_dec.
 From Cava Require Import Arrow.ArrowKind Arrow.ExprSyntax.
-(* From Arrow Require Import Category Arrow Kappa. *)
 
 Import ListNotations.
 
 Set Implicit Arguments.
 Set Asymmetric Patterns.
-
-(* Section Arrow. *)
-  (* Context `{arrow: Arrow}. *)
 
   Section Equivalence.
     Inductive obj_tup : Type := obj_pair : Kind -> Kind -> obj_tup.
@@ -25,41 +21,45 @@ Set Asymmetric Patterns.
       In (vars (obj_pair i o) (pair n1 n2)) E
       -> kappa_equivalence E (Var n1) (Var n2)
 
-    | Abs_equiv : forall x y z 
-      (f1: var1 Unit x -> kappa var1 y z) 
-      (f2: var2 Unit x -> kappa var2 y z) 
+    | Abs_equiv : forall x y z
+      (f1: var1 Unit x -> kappa var1 y z)
+      (f2: var2 Unit x -> kappa var2 y z)
       (E: ctxt),
       (forall n1 n2, kappa_equivalence (vars (obj_pair Unit x) (pair n1 n2) :: E) (f1 n1) (f2 n2))
       -> kappa_equivalence E (Abs f1) (Abs f2)
 
-    | App_equiv : forall E x y z 
-      (f1 : kappa var1 (Tuple x y) z) 
-      (f2 : kappa var2 (Tuple x y) z) 
+    | App_equiv : forall E x y z
+      (f1 : kappa var1 (Tuple x y) z)
+      (f2 : kappa var2 (Tuple x y) z)
       e1 e2,
       kappa_equivalence E f1 f2
       -> kappa_equivalence E e1 e2
       -> kappa_equivalence E (App f1 e1) (App f2 e2)
 
-    | Compose_equiv : forall E x y z 
+    | Compose_equiv : forall E x y z
       (f1: kappa var1 y z) (f2: kappa var2 y z)
       (g1: kappa var1 x y) (g2: kappa var2 x y),
       kappa_equivalence E f1 f2
       -> kappa_equivalence E g1 g2
       -> kappa_equivalence E (Comp f1 g1) (Comp f2 g2)
 
-    (* | Morph_equiv : forall x y E (m: morphism x y), kappa_equivalence E (Morph m) (Morph m) *)
+    | Prim_equiv : forall E p, kappa_equivalence E (ExprSyntax.Primitive p) (ExprSyntax.Primitive p)
 
-    | Letrec_equiv : forall x y z 
-      (v1: var1 Unit x -> kappa var1 Unit x) 
-      (v2: var2 Unit x -> kappa var2 Unit x) 
-      (f1: var1 Unit x -> kappa var1 y z) 
-      (f2: var2 Unit x -> kappa var2 y z) 
+    | Letrec_equiv : forall x y z
+      (v1: var1 Unit x -> kappa var1 Unit x)
+      (v2: var2 Unit x -> kappa var2 Unit x)
+      (f1: var1 Unit x -> kappa var1 y z)
+      (f2: var2 Unit x -> kappa var2 y z)
       (E: ctxt),
       (forall n1 n2, kappa_equivalence (vars (obj_pair Unit x) (pair n1 n2) :: E) (v1 n1) (v2 n2))
-      -> 
+      ->
       (forall n1 n2, kappa_equivalence (vars (obj_pair Unit x) (pair n1 n2) :: E) (f1 n1) (f2 n2))
-      -> 
-      kappa_equivalence E (LetRec v1 f1) (LetRec v2 f2).
+      ->
+      kappa_equivalence E (LetRec v1 f1) (LetRec v2 f2)
+
+    | Id_equiv : forall x E, kappa_equivalence E (@Id var1 x) (Id var2)
+    .
+
   End Equivalence.
 
   Definition Wf {i o} (e: Kappa i o) := forall var1 var2, kappa_equivalence [] (e var1) (e var2).
