cava/cava/Cava/Arrow/ExprSyntax.v
@@ -10,9 +10,6 @@ Set Implicit Arguments.
 Set Asymmetric Patterns.
 
 Section vars.
-  (* Context `{arrow: Arrow}. *)
-
-  (* Notation Kind_pair := (Kind * Kind)%type. *)
   Definition natvar : Kind -> Kind -> Type := fun _ _ => nat.
   Definition unitvar : Kind -> Kind -> Type := fun _ _ => unit.
 
@@ -24,20 +21,17 @@ Section vars.
     | Abs : forall {x y z}, (var Unit x -> kappa y z) -> kappa (Tuple x y) z
     | App : forall {x y z}, kappa (Tuple x y) z -> kappa Unit x -> kappa y z
     | Comp: forall {x y z}, kappa y z -> kappa x y -> kappa x z
-    (* | Morph : forall {x y}, morphism x y -> kappa x y *)
-    | Primitive : forall prim, kappa (primitive_input prim) (primitive_output prim) 
+    | Primitive : forall prim, kappa (primitive_input prim) (primitive_output prim)
     | Let: forall {x y z}, kappa Unit x -> (var Unit x -> kappa y z) -> kappa y z
     | LetRec : forall {x y z}, (var Unit x -> kappa Unit x) -> (var Unit x -> kappa y z) -> kappa y z
-    
     | Id : forall {x}, kappa x x
     .
-
   End Vars.
 
-  Fixpoint reverse_nth {A} (l: list A) (n: nat) {struct l}: option A := 
+  Fixpoint reverse_nth {A} (l: list A) (n: nat) {struct l}: option A :=
     match l with
     | [] => None
-    | x :: xs => 
+    | x :: xs =>
       match eq_nat_dec n (length xs) with
       | left _ => Some x
       | right Hneq => reverse_nth xs n
@@ -53,149 +47,24 @@ Section vars.
     match expr with
     | Var _ _ n  => ok_lookup ctxt n o
     | Abs x _ _ f => wf_phoas_context (x :: ctxt) (f (length ctxt))
-    | App _ _ _ e1 e2 => wf_phoas_context ctxt e1 /\ wf_phoas_context ctxt e2 
+    | App _ _ _ e1 e2 => wf_phoas_context ctxt e1 /\ wf_phoas_context ctxt e2
     | Comp _ _ _ e1 e2 => wf_phoas_context ctxt e1 /\ wf_phoas_context ctxt e2
-    (* | Morph _ _ _ => True *)
     | Primitive _ => True
     | Id _ => True
-    | Let x _ _ v f => wf_phoas_context (x :: ctxt) (f (length ctxt)) /\ wf_phoas_context ctxt v 
+    | Let x _ _ v f => wf_phoas_context (x :: ctxt) (f (length ctxt)) /\ wf_phoas_context ctxt v
     | LetRec x _ _ v f => wf_phoas_context (x :: ctxt) (v (length ctxt)) /\ wf_phoas_context (x :: ctxt) (f (length ctxt))
     end.
 
-  (* Section ctxt.
-    Context {ctxt: list Kind}.
-  
-    Lemma wf_phoas_context_lax_abs: forall {x y z} f,
-      @wf_phoas_context (Tuple x y) z ctxt (Abs f) -> @wf_phoas_context y z (x :: ctxt) (f (length ctxt)).
-    Proof. auto. Qed.
-
-    Hint Extern 10 => 
-      match goal with
-      | [H: wf_phoas_context (_ :: ?ctxt) (Var _ ?v) |- _] => 
-        unfold wf_phoas_context, reverse_nth in H;
-        destruct (PeanoNat.Nat.eq_dec v (length ctxt))
-      | [H: wf_phoas_context _ _ |- _] => inversion H
-      end : core.
-  
-    Lemma wf_phoas_context_lax_var: forall {x y a} v ,
-      wf_phoas_context (i:=x) (o:=y) (a :: ctxt) (Var _ v) -> wf_phoas_context ctxt (Var _ v) \/ v = length ctxt.
-    Proof. auto. Qed.
-  
-    Lemma wf_phoas_context_lax_compose1: forall {x y z} e1 e2,
-      @wf_phoas_context x z ctxt (Comp e2 e1) -> @wf_phoas_context x y ctxt e1.
-    Proof. auto. Qed.
-  
-    Lemma wf_phoas_context_lax_compose2: forall {x y z} e1 e2,
-      @wf_phoas_context x z ctxt (Comp e2 e1) -> @wf_phoas_context y z ctxt e2.
-    Proof. auto. Qed.
-  
-    Lemma wf_phoas_context_lax_app1: forall {x y z} f e,
-      wf_phoas_context ctxt (App f e) -> @wf_phoas_context (Tuple x y) z ctxt f.
-    Proof. auto. Qed.
-  
-    Lemma wf_phoas_context_lax_app2: forall {x y z} f e,
-    Proof. auto. Qed.
-      @wf_phoas_context y z ctxt (App f e) -> @wf_phoas_context u x ctxt e.
-
-    Lemma wf_phoas_context_lax_let1: forall {x y z} v f,
-      @wf_phoas_context y z ctxt (Let v f)
-      -> @wf_phoas_context u x ctxt v.
-    Proof. auto. Qed.
-
-    Lemma wf_phoas_context_lax_let2: forall {x y z} v f,
-      @wf_phoas_context y z ctxt (Let (x:=x) v f)
-      -> @wf_phoas_context y z (x :: ctxt) (f (length ctxt)).
-    Proof. auto. Qed.
-  
-    Lemma wf_phoas_context_lax_letrec1: forall {x y z} v f,
-      @wf_phoas_context y z ctxt (LetRec v f)
-      -> @wf_phoas_context u x (x :: ctxt) (v (length ctxt)).
-    Proof. auto. Qed.
-  
-    Lemma wf_phoas_context_lax_letrec2: forall {x y z} v f,
-      @wf_phoas_context y z ctxt (LetRec (x:=x) v f)
-      -> @wf_phoas_context y z (x :: ctxt) (f (length ctxt)).
-    Proof. auto. Qed.
-  End ctxt.
-
-  Fixpoint wf_phoas_context_elim {i o}
-    (ctxt: list Kind)
-    (expr: kappa natvar i o) {struct expr}
-    : Prop :=
-    match expr with
-    | Var _ _ n  => ok_lookup ctxt n o
-    | Abs x _ _ f => wf_phoas_context_elim (x :: ctxt) (f (length ctxt))
-    | App _ _ _ e1 e2 => forall (p: Prop),
-      (wf_phoas_context_elim ctxt e1 -> wf_phoas_context_elim ctxt e2 -> p) -> p
-    | Comp _ _ _ e1 e2 => forall (p: Prop),
-      (wf_phoas_context_elim ctxt e1 -> wf_phoas_context_elim ctxt e2 -> p) -> p
-    | Morph _ _ _ => True
-    | Let x _ _ v f => forall (p: Prop), 
-      (wf_phoas_context_elim ctxt v -> wf_phoas_context_elim (x :: ctxt) (f (length ctxt)) -> p) -> p
-    | LetRec x _ _ v f => forall (p: Prop),
-      (wf_phoas_context_elim (x :: ctxt) (v (length ctxt))
-      -> wf_phoas_context_elim (x :: ctxt) (f (length ctxt)) -> p) -> p
-    end.
-
-  Goal forall x, wf_phoas_context [] (Abs (x:=x) (y:=u) (z:=x) (fun x => Let (Var _ x) (fun y => Var _ y))).
-  Proof. cbn; auto. Qed.
-  Goal forall x, wf_phoas_context_elim [] (Abs (x:=x) (y:=u) (z:=x) (fun x => Let (Var _ x) (fun y => Var _ y))).
-  Proof. cbn; auto. Qed.
-
-  Lemma phoas_context_elim {i o} (expr: kappa natvar i o): forall (ctxt: list Kind),
-    wf_phoas_context_elim ctxt expr -> wf_phoas_context ctxt expr.
-  Proof.
-    induction expr; cbn [wf_phoas_context_elim] in *; 
-      simpl; intros;
-      try constructor;
-      try apply H;
-      try apply H0;
-      try apply H1;
-      auto.
-  Qed.
-
-  Lemma wf_let_is_wf_app_abs {x i o}
-    (v: kappa natvar u x)
-    (f: natvar u x -> kappa natvar i o)
-    : forall (ctxt: list Kind), wf_phoas_context ctxt (Let v f) -> wf_phoas_context ctxt (App (Abs f) v).
-  Proof. now cbn. Qed. *)
-
   Definition Kappa i o := forall var, kappa var i o.
-
-  (* common functions *)
-
-  (* Open Scope category_scope.
-  Context {arrow_drop: ArrowDrop arrow}. *)
-
-  (* Definition kappa_fst {var x y}: kappa var (product (product x y) u) x := 
-    Morph var (cancelr >>> second drop >>> cancelr).
-  Definition kappa_snd {var x y}: kappa var (product (product x y) u) y := 
-    Morph var (cancelr >>> first drop >>> cancell).
-  Definition kappa_pair {var x y}: kappa var (product x (product y u)) (product x y) := 
-    Morph var (second cancelr). *)
 
 End vars.
 
-(* Ltac dispatch_wf_phoas_context := 
-  apply phoas_context_elim;
-  lazy -[reverse_nth];
-  repeat lazymatch goal with
-  | [ |- True ] => constructor
-  | [ |- forall p, (?H1 -> ?H2 -> p) -> p ] => 
-    let x := fresh in (let y := fresh in (
-      intros x y; apply y; clear x y
-    ))
-  end; 
-  repeat lazymatch goal with
-  | [ |- reverse_nth _ _ = Some _] => exact eq_refl
-  end.  *)
 Print Var.
 Arguments Var {var _ _}.
 Arguments Abs {var _ _ _}.
 Arguments App {var _ _ _}.
 Arguments Comp {var _ _ _}.
 Arguments Primitive {var}.
-(* Arguments Kappa.Morph {_ _ _ _ _ var _ _}. *)
 Arguments LetRec {var _ _ _}.
 
 Instance KappaCat : Category Kind := {
